

1. Consider a forward SDE

$$dx_t = f(x_t, t) dt + g(x_t, t) dW_t,$$

show that the corresponding probability flow ODE is written as

$$dx_t = \left[f(x_t, t) - \frac{\partial}{\partial x} g^2(x_t, t) - \frac{g^2(x_t, t)}{2} \frac{\partial}{\partial x} \log p(x_t, t) \right] dt. \quad \text{--- } \textcircled{*}$$

By Fokker-Planck Equation: $\frac{\partial p(x,t)}{\partial t} = -\frac{\partial}{\partial x} [f(x,t)p(x,t)] + \frac{1}{2} \frac{\partial^2}{\partial x^2} [g^2(x,t)p(x,t)]$

This eqn is a form of conti. eqn. $\frac{\partial p}{\partial t} = -\frac{\partial J_{SDE}}{\partial x}$, where J_{SDE} is the probability current of the stochastic process. By factoring the FPE, we can identify this current:

$$J_{SDE}(x, t) = f(x, t)p(x, t) - \frac{1}{2} \frac{\partial}{\partial x} [g^2(x, t)p(x, t)] \quad \text{--- } \textcircled{*}$$

Let $\textcircled{*}$ becomes to $dx_t = v(x, t) dt \quad \text{--- } \textcircled{\circ}$, which $v(x, t) = f(x, t) - \frac{\partial}{\partial x} g^2(x, t) - \frac{g^2(x, t)}{2} \frac{\partial}{\partial x} \log p(x, t)$

The evolution of a density $p(x, t)$ under this deterministic flow is given by the standard Continuity Eqn: $\frac{\partial p(x, t)}{\partial t} = -\frac{\partial}{\partial x} [v(x, t)p(x, t)]$

The probability current J_{ODE} for this flow is simply: $J_{ODE}(x, t) = v(x, t)p(x, t) \quad \text{--- } \textcircled{\times}$

For the $\textcircled{\circ}$ to be the "probability flow" corresponding to the $\textcircled{*}$, they must both describe the exact same probability density evolution $p(x, t)$. This means their $\frac{\partial p}{\partial t}$ terms must be identical, which implies their probability currents must be equal. $J_{SDE} = J_{ODE}$

Subst. $\textcircled{*}$ and $\textcircled{\times}$:

$$f(x, t)p(x, t) - \frac{1}{2} \frac{\partial}{\partial x} [g^2(x, t)p(x, t)] = v(x, t)p(x, t)$$

$$\Rightarrow \quad vp = fp - \frac{1}{2} \frac{\partial}{\partial x} (g^2 p)$$

$$\Rightarrow \quad v = f - \frac{1}{2p} \frac{\partial}{\partial x} (g^2 p)$$

$$\Rightarrow \quad \frac{\partial}{\partial x} (g^2 p) = \left(\frac{\partial g^2}{\partial x} \right) p + g^2 \left(\frac{\partial p}{\partial x} \right)$$

$$\Rightarrow \quad v = f - \frac{1}{2p} \left[\left(\frac{\partial g^2}{\partial x} \right) p + g^2 \left(\frac{\partial p}{\partial x} \right) \right]$$

$$\Rightarrow \quad v = f - \frac{1}{2} \frac{\partial g^2}{\partial x} - \frac{g^2}{2} \left(\frac{1}{p} \frac{\partial p}{\partial x} \right)$$

$$\frac{\partial}{\partial x} \log p(x, t) = \frac{1}{p(x, t)} \frac{\partial p(x, t)}{\partial x}$$

$$\text{, then } v = f - \frac{1}{2} \frac{\partial g^2}{\partial x} - \frac{g^2}{2} \frac{\partial}{\partial x} \log p$$

$$v(x, t) = f(x, t) - \frac{1}{2} \frac{\partial}{\partial x} g^2(x, t) - \frac{g^2(x, t)}{2} \frac{\partial}{\partial x} \log p(x, t)$$

$$\text{Hence, } dx_t = \left[f(x_t, t) - \frac{1}{2} \frac{\partial}{\partial x} g^2(x_t, t) - \frac{g^2(x_t, t)}{2} \frac{\partial}{\partial x} \log p(x_t, t) \right] dt \quad \#$$